thys/Registers/Axioms_Complement_Quantum.thy
@@ -549,4 +549,428 @@ lemma complement_unique:
   shows \<open>equivalent_registers G H\<close>
   by (metis assms compatible_def complement_range same_range_equivalent)
 
+
+
+
+
+
+
+
+
+
+
+
+
+
+
+
+
+subsection \<open>Finite dimensional complement\<close>
+
+typedef ('a, 'b::finite) complement_domain = \<open>{..< if CARD('b) div CARD('a) \<noteq> 0 then CARD('b) div CARD('a) else 1}\<close>
+  by auto
+
+instance complement_domain :: (type, finite) finite
+proof intro_classes
+  have \<open>inj Rep_complement_domain\<close>
+    by (simp add: Rep_complement_domain_inject inj_on_def)
+  moreover have \<open>finite (range Rep_complement_domain)\<close>
+    by (metis finite_lessThan type_definition.Rep_range type_definition_complement_domain)
+  ultimately show \<open>finite (UNIV :: ('a,'b) complement_domain set)\<close>
+    using finite_image_iff by blast
+qed
+
+lemma CARD_complement_domain: 
+  assumes \<open>CARD('b::finite) = n * CARD('a)\<close>
+  shows \<open>CARD(('a,'b) complement_domain) = n\<close>
+proof -
+  from assms have \<open>n > 0\<close>
+    by (metis nat_0_less_mult_iff zero_less_card_finite)
+  have *: \<open>inj Rep_complement_domain\<close>
+    by (simp add: Rep_complement_domain_inject inj_on_def)
+  moreover have \<open>card (range (Rep_complement_domain :: ('a,'b) complement_domain \<Rightarrow> _)) = n\<close>
+    apply (subst type_definition.Rep_range[OF type_definition_complement_domain])
+    using assms \<open>n > 0\<close> apply simp
+    by force
+  ultimately show ?thesis
+    by (metis card_image)
+qed
+
+lemma register_decomposition_finite_aux:
+  fixes \<Phi> :: \<open>'a::finite update \<Rightarrow> 'b::finite update\<close>
+  assumes [simp]: \<open>register \<Phi>\<close>
+  shows \<open>\<exists>U :: ('a \<times> ('a, 'b) complement_domain) ell2 \<Rightarrow>\<^sub>C\<^sub>L 'b ell2. unitary U \<and> 
+              (\<forall>\<theta>. \<Phi> \<theta> = sandwich U (\<theta> \<otimes>\<^sub>o id_cblinfun))\<close>
+  \<comment> \<open>Proof based on @{cite daws21unitalanswer}\<close>
+proof -
+  note [[simproc del: compatibility_warn]]
+  fix \<xi>0 :: 'a
+
+  have [simp]: \<open>clinear \<Phi>\<close>
+    by (simp add: clinear_register)
+
+  define P where \<open>P i = Proj (ccspan {ket i})\<close> for i :: 'a
+  have P_butter: \<open>P i = selfbutterket i\<close> for i
+    by (simp add: P_def butterfly_eq_proj)
+
+  define P' where \<open>P' i = \<Phi> (P i)\<close> for i :: 'a
+  have proj_P': \<open>is_Proj (P' i)\<close> for i
+    by (simp add: P_def P'_def register_projector)
+  have \<open>(\<Sum>i\<in>UNIV. P i) = id_cblinfun\<close>
+    using sum_butterfly_ket P_butter by simp
+  then have sumP'id: \<open>(\<Sum>i\<in>UNIV. P' i) = id_cblinfun\<close>
+    unfolding P'_def 
+    apply (subst complex_vector.linear_sum[OF \<open>clinear \<Phi>\<close>, symmetric])
+    by auto
+
+  define S where \<open>S i = P' i *\<^sub>S \<top>\<close> for i :: 'a
+  have P'id: \<open>P' i *\<^sub>V \<psi> = \<psi>\<close> if \<open>\<psi> \<in> space_as_set (S i)\<close> for i \<psi>
+    using S_def that proj_P'
+    by (metis cblinfun_fixes_range is_Proj_algebraic)
+
+  obtain B0 where finiteB0: \<open>finite (B0 i)\<close> and cspanB0: \<open>cspan (B0 i) = space_as_set (S i)\<close> for i
+    apply atomize_elim apply (simp flip: all_conj_distrib) apply (rule choice)
+    by (meson cfinite_dim_finite_subspace_basis csubspace_space_as_set)
+
+  obtain B where orthoB: \<open>is_ortho_set (B i)\<close>
+    and normalB: \<open>\<And>b. b \<in> B i \<Longrightarrow> norm b = 1\<close>
+    and cspanB: \<open>cspan (B i) = cspan (B0 i)\<close>
+    and finiteB: \<open>finite (B i)\<close> for i
+    apply atomize_elim apply (simp flip: all_conj_distrib) apply (rule choice)
+    using orthonormal_basis_of_cspan[OF finiteB0] by blast
+
+  from cspanB cspanB0 have cspanB: \<open>cspan (B i) = space_as_set (S i)\<close> for i
+    by simp
+  then have ccspanB: \<open>ccspan (B i) = S i\<close> for i
+    by (metis ccspan.rep_eq closure_finite_cspan finiteB space_as_set_inject)
+  from orthoB have indepB: \<open>cindependent (B i)\<close> for i
+    by (simp add: Complex_Inner_Product.is_ortho_set_cindependent)
+
+  have orthoBiBj: \<open>is_orthogonal x y\<close> if \<open>x \<in> B i\<close> and \<open>y \<in> B j\<close> and \<open>i \<noteq> j\<close> for x y i j
+  proof -
+    from \<open>x \<in> B i\<close> obtain x' where x: \<open>x = P' i *\<^sub>V x'\<close>
+      by (metis S_def cblinfun_fixes_range complex_vector.span_base cspanB is_Proj_idempotent proj_P')
+    from \<open>y \<in> B j\<close> obtain y' where y: \<open>y = P' j *\<^sub>V y'\<close>
+      by (metis S_def cblinfun_fixes_range complex_vector.span_base cspanB is_Proj_idempotent proj_P')
+    have \<open>cinner x y = cinner (P' i *\<^sub>V x') (P' j *\<^sub>V  y')\<close>
+      using x y by simp
+    also have \<open>\<dots> = cinner (P' j *\<^sub>V P' i *\<^sub>V x') y'\<close>
+      by (metis cinner_adj_left is_Proj_algebraic proj_P')
+    also have \<open>\<dots> = cinner (\<Phi> (P j o\<^sub>C\<^sub>L P i) *\<^sub>V x') y'\<close>
+      unfolding P'_def register_mult[OF \<open>register \<Phi>\<close>, symmetric] by simp
+    also have \<open>\<dots> = cinner (\<Phi> (selfbutterket j o\<^sub>C\<^sub>L selfbutterket i) *\<^sub>V x') y'\<close>
+      unfolding P_butter by simp
+    also have \<open>\<dots> = cinner (\<Phi> 0 *\<^sub>V x') y'\<close>
+      by (metis butterfly_comp_butterfly complex_vector.scale_eq_0_iff orthogonal_ket that(3))
+    also have \<open>\<dots> = 0\<close>
+      by (simp add: complex_vector.linear_0)
+    finally show ?thesis
+      by -
+  qed
+
+
+  define B' where \<open>B' = (\<Union>i\<in>UNIV. B i)\<close>
+
+  have P'B: \<open>P' i = Proj (ccspan (B i))\<close> for i
+    unfolding ccspanB S_def
+    using proj_P' Proj_on_own_range'[symmetric] is_Proj_algebraic by blast
+
+  have \<open>(\<Sum>i\<in>UNIV. P' i) = Proj (ccspan B')\<close>
+  proof (unfold B'_def, use finite[of UNIV] in induction)
+    case empty
+    show ?case by auto
+  next
+    case (insert j M)
+    have \<open>(\<Sum>i\<in>insert j M. P' i) = P' j + (\<Sum>i\<in>M. P' i)\<close>
+      by (meson insert.hyps(1) insert.hyps(2) sum.insert)
+    also have \<open>\<dots> = Proj (ccspan (B j)) + Proj (ccspan (\<Union>i\<in>M. B i))\<close>
+      unfolding P'B insert.IH[symmetric] by simp
+    also have \<open>\<dots> = Proj (ccspan (B j \<union> (\<Union>i\<in>M. B i)))\<close>
+      apply (rule Proj_orthog_ccspan_union[symmetric])
+      using orthoBiBj insert.hyps(2) by auto
+    also have \<open>\<dots> = Proj (ccspan (\<Union>i\<in>insert j M. B i))\<close>
+      by auto
+    finally show ?case
+      by simp
+  qed
+
+  with sumP'id 
+  have ccspanB': \<open>ccspan B' = \<top>\<close>
+    by (metis Proj_range cblinfun_image_id)
+  hence cspanB': \<open>cspan B' = UNIV\<close>
+    by (metis B'_def finiteB ccspan.rep_eq finite_UN_I finite_class.finite_UNIV closure_finite_cspan top_ccsubspace.rep_eq)
+
+  from orthoBiBj orthoB have orthoB': \<open>is_ortho_set B'\<close>
+    unfolding B'_def is_ortho_set_def by blast
+  then have indepB': \<open>cindependent B'\<close>
+    using is_ortho_set_cindependent by blast
+  have cardB': \<open>card B' = CARD('b)\<close>
+    apply (subst complex_vector.dim_span_eq_card_independent[symmetric])
+     apply (rule indepB')
+    apply (subst cspanB')
+    using cdim_UNIV_ell2 by auto
+
+  from orthoBiBj orthoB
+  have Bdisj: \<open>B i \<inter> B j = {}\<close> if \<open>i \<noteq> j\<close> for i j
+    unfolding is_ortho_set_def
+    apply auto by (metis cinner_eq_zero_iff that)
+
+  have cardBsame: \<open>card (B i) = card (B j)\<close> for i j
+  proof -
+    define Si_to_Sj where \<open>Si_to_Sj i j \<psi> = \<Phi> (butterket j i) *\<^sub>V \<psi>\<close> for i j \<psi>
+    have S2S2S: \<open>Si_to_Sj j i (Si_to_Sj i j \<psi>) = \<psi>\<close> if \<open>\<psi> \<in> space_as_set (S i)\<close> for i j \<psi>
+      using that P'id
+      by (simp add: Si_to_Sj_def cblinfun_apply_cblinfun_compose[symmetric] register_mult P_butter P'_def)
+    also have lin[simp]: \<open>clinear (Si_to_Sj i j)\<close> for i j
+      unfolding Si_to_Sj_def by simp
+    have S2S: \<open>Si_to_Sj i j x \<in> space_as_set (S j)\<close> for i j x
+    proof -
+      have \<open>Si_to_Sj i j x = P' j *\<^sub>V Si_to_Sj i j x\<close>
+        by (simp add: Si_to_Sj_def cblinfun_apply_cblinfun_compose[symmetric] register_mult P_butter P'_def)
+      also have \<open>P' j *\<^sub>V Si_to_Sj i j x \<in> space_as_set (S j)\<close>
+        by (simp add: S_def)
+      finally show ?thesis by -
+    qed
+    have bij: \<open>bij_betw (Si_to_Sj i j) (space_as_set (S i)) (space_as_set (S j))\<close>
+      apply (rule bij_betwI[where g=\<open>Si_to_Sj j i\<close>])
+      using S2S S2S2S by (auto intro!: funcsetI)
+    have \<open>cdim (space_as_set (S i)) = cdim (space_as_set (S j))\<close>
+      using lin apply (rule isomorphic_equal_cdim[where f=\<open>Si_to_Sj i j\<close>])
+      using bij apply (auto simp: bij_betw_def)
+      by (metis complex_vector.span_span cspanB)
+    then show ?thesis
+      by (metis complex_vector.dim_span_eq_card_independent cspanB indepB)
+  qed
+
+  have CARD'b: \<open>CARD('b) = card (B \<xi>0) * CARD('a)\<close>
+  proof -
+    have \<open>CARD('b) = card B'\<close>
+      using cardB' by simp
+    also have \<open>\<dots> = (\<Sum>i\<in>UNIV. card (B i))\<close>
+      unfolding B'_def apply (rule card_UN_disjoint)
+      using finiteB Bdisj by auto
+    also have \<open>\<dots> = (\<Sum>(i::'a)\<in>UNIV. card (B \<xi>0))\<close>
+      using cardBsame by metis
+    also have \<open>\<dots> = card (B \<xi>0) * CARD('a)\<close>
+      by auto
+    finally show ?thesis by -
+  qed
+
+  obtain f where bij_f: \<open>bij_betw f (UNIV::('a,'b) complement_domain set) (B \<xi>0)\<close>
+    apply atomize_elim apply (rule finite_same_card_bij)
+    using finiteB CARD_complement_domain[OF CARD'b] by auto
+
+  define u where \<open>u = (\<lambda>(\<xi>,\<alpha>). \<Phi> (butterket \<xi> \<xi>0) *\<^sub>V f \<alpha>)\<close> for \<xi> :: 'a and \<alpha> :: \<open>('a,'b) complement_domain\<close>
+  obtain U where Uapply: \<open>U *\<^sub>V ket \<xi>\<alpha> = u \<xi>\<alpha>\<close> for \<xi>\<alpha>
+    apply atomize_elim
+    apply (rule exI[of _ \<open>cblinfun_extension (range ket) (\<lambda>k. u (inv ket k))\<close>])
+    apply (subst cblinfun_extension_apply)
+      apply (rule cblinfun_extension_exists_finite_dim)
+    by (auto simp add: inj_ket cindependent_ket)
+
+  define eqa where \<open>eqa a b = (if a = b then 1 else 0 :: complex)\<close> for a b :: 'a
+  define eqc where \<open>eqc a b = (if a = b then 1 else 0 :: complex)\<close> for a b :: \<open>('a,'b) complement_domain\<close>
+  define eqac where \<open>eqac a b = (if a = b then 1 else 0 :: complex)\<close> for a b :: \<open>'a * ('a,'b) complement_domain\<close>
+
+  have \<open>cinner (U *\<^sub>V ket \<xi>\<alpha>) (U *\<^sub>V ket \<xi>'\<alpha>') = eqac \<xi>\<alpha> \<xi>'\<alpha>'\<close> for \<xi>\<alpha> \<xi>'\<alpha>'
+  proof -
+    obtain \<xi> \<alpha> \<xi>' \<alpha>' where \<xi>\<alpha>: \<open>\<xi>\<alpha> = (\<xi>,\<alpha>)\<close> and \<xi>'\<alpha>': \<open>\<xi>'\<alpha>' = (\<xi>',\<alpha>')\<close>
+      apply atomize_elim by auto
+    have \<open>cinner (U *\<^sub>V ket (\<xi>,\<alpha>)) (U *\<^sub>V ket (\<xi>', \<alpha>')) = cinner (\<Phi> (butterket \<xi> \<xi>0) *\<^sub>V f \<alpha>) (\<Phi> (butterket \<xi>' \<xi>0) *\<^sub>V f \<alpha>')\<close>
+      unfolding Uapply u_def by simp
+    also have \<open>\<dots> = cinner ((\<Phi> (butterket \<xi>' \<xi>0))* *\<^sub>V \<Phi> (butterket \<xi> \<xi>0) *\<^sub>V f \<alpha>) (f \<alpha>')\<close>
+      by (simp add: cinner_adj_left)
+    also have \<open>\<dots> = cinner (\<Phi> (butterket \<xi>' \<xi>0 *) *\<^sub>V \<Phi> (butterket \<xi> \<xi>0) *\<^sub>V f \<alpha>) (f \<alpha>')\<close>
+      by (metis (no_types, lifting) assms register_def)
+    also have \<open>\<dots> = cinner (\<Phi> (butterket \<xi>0 \<xi>' o\<^sub>C\<^sub>L butterket \<xi> \<xi>0) *\<^sub>V f \<alpha>) (f \<alpha>')\<close>
+      by (simp add: register_mult cblinfun_apply_cblinfun_compose[symmetric])
+    also have \<open>\<dots> = cinner (\<Phi> (eqa \<xi>' \<xi> *\<^sub>C selfbutterket \<xi>0) *\<^sub>V f \<alpha>) (f \<alpha>')\<close>
+      apply simp by (metis eqa_def cinner_ket)
+    also have \<open>\<dots> = eqa \<xi>' \<xi> * cinner (\<Phi> (selfbutterket \<xi>0) *\<^sub>V f \<alpha>) (f \<alpha>')\<close>
+      by (smt (verit, ccfv_threshold) \<open>clinear \<Phi>\<close> eqa_def cblinfun.scaleC_left cinner_commute 
+              cinner_scaleC_left cinner_zero_right complex_cnj_one complex_vector.linear_scale)
+    also have \<open>\<dots> = eqa \<xi>' \<xi> * cinner (P' \<xi>0 *\<^sub>V f \<alpha>) (f \<alpha>')\<close>
+      using P_butter P'_def by simp
+    also have \<open>\<dots> = eqa \<xi>' \<xi> * cinner (f \<alpha>) (f \<alpha>')\<close>
+      apply (subst P'id)
+       apply (metis bij_betw_imp_surj_on bij_f complex_vector.span_base cspanB rangeI)
+      by simp
+    also have \<open>\<dots> = eqa \<xi>' \<xi> * eqc \<alpha> \<alpha>'\<close>
+      using bij_f orthoB normalB unfolding is_ortho_set_def eqc_def apply auto
+       apply (metis bij_betw_imp_surj_on cnorm_eq_1 rangeI)
+      by (smt (z3) bij_betw_iff_bijections iso_tuple_UNIV_I)
+    finally show ?thesis
+      by (simp add: eqa_def eqac_def eqc_def \<xi>'\<alpha>' \<xi>\<alpha>)
+  qed
+  then have [simp]: \<open>isometry U\<close>
+    apply (rule_tac orthogonal_on_basis_is_isometry[where B=\<open>range ket\<close>])
+    using eqac_def by auto
+
+  have \<open>sandwich (U*) (\<Phi> (butterket \<xi> \<eta>)) = butterket \<xi> \<eta> \<otimes>\<^sub>o id_cblinfun\<close> for \<xi> \<eta>
+  proof (rule equal_ket, rename_tac \<xi>1\<alpha>)
+    fix \<xi>1\<alpha> obtain \<xi>1 :: 'a and \<alpha> :: \<open>('a,'b) complement_domain\<close> where \<xi>1\<alpha>: \<open>\<xi>1\<alpha> = (\<xi>1,\<alpha>)\<close> 
+      apply atomize_elim by auto
+    have \<open>sandwich (U*) (\<Phi> (butterket \<xi> \<eta>)) *\<^sub>V ket \<xi>1\<alpha> = U* *\<^sub>V \<Phi> (butterket \<xi> \<eta>) *\<^sub>V \<Phi> (butterket \<xi>1 \<xi>0) *\<^sub>V f \<alpha>\<close>
+      by (simp add: sandwich_apply[abs_def] cblinfun_apply_cblinfun_compose \<xi>1\<alpha> Uapply u_def)
+    also have \<open>\<dots> = U* *\<^sub>V \<Phi> (butterket \<xi> \<eta> o\<^sub>C\<^sub>L butterket \<xi>1 \<xi>0) *\<^sub>V f \<alpha>\<close>
+      by (metis (no_types, lifting) assms butterfly_comp_butterfly lift_cblinfun_comp(4) register_mult)
+    also have \<open>\<dots> = U* *\<^sub>V \<Phi> (eqa \<eta> \<xi>1 *\<^sub>C butterket \<xi> \<xi>0) *\<^sub>V f \<alpha>\<close>
+      by (simp add: eqa_def cinner_ket)
+    also have \<open>\<dots> = eqa \<eta> \<xi>1 *\<^sub>C U* *\<^sub>V \<Phi> (butterket \<xi> \<xi>0) *\<^sub>V f \<alpha>\<close>
+      by (simp add: complex_vector.linear_scale)
+    also have \<open>\<dots> = eqa \<eta> \<xi>1 *\<^sub>C U* *\<^sub>V U *\<^sub>V ket (\<xi>, \<alpha>)\<close>
+      unfolding Uapply u_def by simp
+    also from \<open>isometry U\<close> have \<open>\<dots> = eqa \<eta> \<xi>1 *\<^sub>C ket (\<xi>, \<alpha>)\<close>
+      unfolding cblinfun_apply_cblinfun_compose[symmetric] by simp
+    also have \<open>\<dots> = (butterket \<xi> \<eta> *\<^sub>V ket \<xi>1) \<otimes>\<^sub>s ket \<alpha>\<close>
+      by (simp add: eqa_def tensor_ell2_scaleC1 tensor_ell2_ket)
+    also have \<open>\<dots> = (butterket \<xi> \<eta> \<otimes>\<^sub>o id_cblinfun) *\<^sub>V ket \<xi>1\<alpha>\<close>
+      by (simp add: \<xi>1\<alpha> tensor_op_ket)
+    finally show \<open>sandwich (U*) (\<Phi> (butterket \<xi> \<eta>)) *\<^sub>V ket \<xi>1\<alpha> = (butterket \<xi> \<eta> \<otimes>\<^sub>o id_cblinfun) *\<^sub>V ket \<xi>1\<alpha>\<close>
+      by -
+  qed
+  then have 1: \<open>sandwich (U*) (\<Phi> \<theta>) = \<theta> \<otimes>\<^sub>o id_cblinfun\<close> for \<theta>
+    apply (rule clinear_eq_butterfly_ketI[THEN fun_cong, where x=\<theta>, rotated -1])
+    by (auto intro: bounded_clinear.clinear bounded_linear_intros register_bounded_clinear \<open>register \<Phi>\<close>)
+
+  have [simp]: \<open>unitary U\<close>
+  proof -
+    have \<open>\<Phi> (butterket \<xi> \<xi>1) *\<^sub>S \<top> \<le> U *\<^sub>S \<top>\<close> for \<xi> \<xi>1
+    proof -
+      have *: \<open>\<Phi> (butterket \<xi> \<xi>0) *\<^sub>V b \<in> space_as_set (U *\<^sub>S \<top>)\<close> if \<open>b \<in> B \<xi>0\<close> for b
+        apply (subst asm_rl[of \<open>\<Phi> (butterket \<xi> \<xi>0) *\<^sub>V b = u (\<xi>, inv f b)\<close>])
+         apply (simp add: u_def, metis bij_betw_inv_into_right bij_f that)
+        by (metis Uapply cblinfun_apply_in_image)
+
+      have \<open>\<Phi> (butterket \<xi> \<xi>1) *\<^sub>S \<top> = \<Phi> (butterket \<xi> \<xi>0) *\<^sub>S \<Phi> (butterket \<xi>0 \<xi>0) *\<^sub>S \<Phi> (butterket \<xi>0 \<xi>1) *\<^sub>S \<top>\<close>
+        unfolding cblinfun_compose_image[symmetric] register_mult[OF assms]
+        by simp
+      also have \<open>\<dots> \<le> \<Phi> (butterket \<xi> \<xi>0) *\<^sub>S \<Phi> (butterket \<xi>0 \<xi>0) *\<^sub>S \<top>\<close>
+        by (meson cblinfun_image_mono top_greatest)
+      also have \<open>\<dots> = \<Phi> (butterket \<xi> \<xi>0) *\<^sub>S S \<xi>0\<close>
+        by (simp add: S_def P'_def P_butter)
+      also have \<open>\<dots> = \<Phi> (butterket \<xi> \<xi>0) *\<^sub>S ccspan (B \<xi>0)\<close>
+        by (simp add: ccspanB)
+      also have \<open>\<dots> = ccspan (\<Phi> (butterket \<xi> \<xi>0) ` B \<xi>0)\<close>
+        by (meson cblinfun_image_ccspan)
+      also have \<open>\<dots> \<le> U *\<^sub>S \<top>\<close>
+        by (rule ccspan_leqI, use * in auto)
+      finally show ?thesis by -
+    qed
+    moreover have \<open>\<Phi> id_cblinfun *\<^sub>S \<top> \<le> (SUP \<xi>\<in>UNIV. \<Phi> (selfbutterket \<xi>) *\<^sub>S \<top>)\<close>
+      unfolding sum_butterfly_ket[symmetric]
+      apply (subst complex_vector.linear_sum, simp)
+      by (rule cblinfun_sum_image_distr)
+    ultimately have \<open>\<Phi> id_cblinfun *\<^sub>S \<top> \<le> U *\<^sub>S \<top>\<close>
+      apply auto by (meson SUP_le_iff order.trans)
+    then have \<open>U *\<^sub>S \<top> = \<top>\<close>
+      apply auto
+      using top.extremum_unique by blast
+    with \<open>isometry U\<close> show \<open>unitary U\<close>
+      by (rule surj_isometry_is_unitary)
+  qed
+
+  have \<open>\<Phi> \<theta> = sandwich U (\<theta> \<otimes>\<^sub>o id_cblinfun)\<close> for \<theta>
+  proof -
+    from 1 have \<open>sandwich U (sandwich (U*) *\<^sub>V \<Phi> \<theta>) = sandwich U (\<theta> \<otimes>\<^sub>o id_cblinfun)\<close>
+      by simp
+    then show ?thesis
+      by (simp add: sandwich_compose flip: cblinfun_apply_cblinfun_compose)
+  qed
+
+  then show ?thesis
+    apply (rule_tac exI[of _ U])
+    by simp
+qed
+
+lemma register_decomposition_finite:
+  fixes \<Phi> :: \<open>'a update \<Rightarrow> 'b::finite update\<close>
+  assumes [simp]: \<open>register \<Phi>\<close>
+  shows \<open>\<exists>U :: ('a \<times> ('a, 'b) complement_domain) ell2 \<Rightarrow>\<^sub>C\<^sub>L 'b ell2. unitary U \<and> 
+              (\<forall>\<theta>. \<Phi> \<theta> = sandwich U (\<theta> \<otimes>\<^sub>o id_cblinfun))\<close>
+proof -
+  fix a\<^sub>0
+  have inj_butterket: \<open>inj (butterket a\<^sub>0 :: 'a \<Rightarrow> 'a update)\<close>
+  proof (rule injI)
+    fix x y :: 'a
+    assume \<open>butterket a\<^sub>0 x = butterket a\<^sub>0 y\<close>
+    then have \<open>butterket a\<^sub>0 x *\<^sub>V ket x = butterket a\<^sub>0 y *\<^sub>V ket x\<close>
+      by simp
+    then show \<open>x = y\<close>
+      apply (cases \<open>x = y\<close>)
+      by (auto simp: cinner_ket)
+  qed
+
+  from cindependent_butterfly_ket
+  have \<open>cindependent (range (butterket a\<^sub>0) :: 'a update set)\<close>
+    apply (subgoal_tac \<open>(range (butterket a\<^sub>0) :: 'a update set) \<subseteq> {butterket i j |i j. True}\<close>)
+    by (auto intro: complex_vector.dependent_mono)
+  then have \<open>cindependent (\<Phi> ` range (butterket a\<^sub>0))\<close>
+    apply (rule complex_vector.linear_independent_injective_image[rotated])
+    by (simp_all add: register_inj clinear_register)
+  then have \<open>finite (\<Phi> ` range (butterket a\<^sub>0))\<close>
+    using cindependent_cfinite_dim_finite by blast
+  then have \<open>finite (range (butterket a\<^sub>0) :: 'a update set)\<close>
+    apply (rule Finite_Set.inj_on_finite[rotated -1, where f=\<Phi>])
+    by (simp_all add: register_inj)
+  then have \<open>finite (UNIV :: 'a set)\<close>
+    apply (rule Finite_Set.inj_on_finite[rotated -1, where f=\<open>butterket a\<^sub>0\<close>])
+     apply (rule inj_butterket)
+    by simp
+  then have \<open>class.finite TYPE('a)\<close>
+    by intro_classes
+  from register_decomposition_finite_aux[unoverload_type 'a, OF this]
+  show ?thesis
+    using assms by metis
+qed
+
+hide_fact register_decomposition_finite_aux
+
+lemma complement_exists_simple:
+  fixes F :: \<open>'a update \<Rightarrow> 'b::finite update\<close>
+  assumes \<open>register F\<close>
+  shows \<open>\<exists>G :: ('a, 'b) complement_domain update \<Rightarrow> 'b update. compatible F G \<and> iso_register (F;G)\<close>
+proof -
+  note [[simproc del: Laws_Quantum.compatibility_warn]]
+  obtain U :: \<open>('a \<times> ('a, 'b) complement_domain) ell2 \<Rightarrow>\<^sub>C\<^sub>L 'b ell2\<close>
+    where [simp]: "unitary U" and F: \<open>F a = sandwich U (a \<otimes>\<^sub>o id_cblinfun)\<close> for a
+    apply atomize_elim using assms by (rule register_decomposition_finite)
+  define G :: \<open>(('a, 'b) complement_domain) update \<Rightarrow> 'b update\<close> where \<open>G b = sandwich U (id_cblinfun \<otimes>\<^sub>o b)\<close> for b
+  have [simp]: \<open>register G\<close>
+    unfolding G_def apply (rule register_decomposition_converse) by simp
+  have \<open>F a o\<^sub>C\<^sub>L G b = G b o\<^sub>C\<^sub>L F a\<close> for a b
+  proof -
+    have \<open>F a o\<^sub>C\<^sub>L G b = sandwich U (a \<otimes>\<^sub>o b)\<close>
+      apply (auto simp: F G_def sandwich_apply)
+      by (metis (no_types, lifting) \<open>unitary U\<close> isometryD cblinfun_assoc_left(1) comp_tensor_op cblinfun_compose_id_right cblinfun_compose_id_left unitary_isometry)
+    moreover have \<open>G b o\<^sub>C\<^sub>L F a = sandwich U (a \<otimes>\<^sub>o b)\<close>
+      apply (auto simp: F G_def sandwich_apply)
+      by (metis (no_types, lifting) \<open>unitary U\<close> isometryD cblinfun_assoc_left(1) comp_tensor_op cblinfun_compose_id_right cblinfun_compose_id_left unitary_isometry)
+    ultimately show ?thesis by simp
+  qed
+  then have [simp]: \<open>compatible F G\<close>
+    by (auto simp: compatible_def \<open>register F\<close> \<open>register G\<close>)
+  moreover have \<open>iso_register (F;G)\<close>
+  proof -
+    have \<open>(F;G) (a \<otimes>\<^sub>o b) = sandwich U (a \<otimes>\<^sub>o b)\<close> for a b
+      apply (auto simp: register_pair_apply F G_def sandwich_apply)
+      by (metis (no_types, lifting) \<open>unitary U\<close> isometryD cblinfun_assoc_left(1) comp_tensor_op cblinfun_compose_id_right cblinfun_compose_id_left unitary_isometry)
+    then have FG: \<open>(F;G) = sandwich U\<close>
+      apply (rule tensor_extensionality[rotated -1])
+      by (simp_all add: bounded_cbilinear.add_left bounded_cbilinear_cblinfun_compose bounded_cbilinear.add_right clinearI unitary_sandwich_register)
+
+    define I where \<open>I = sandwich (U*)\<close> for x
+    have [simp]: \<open>register I\<close>
+      by (simp add: I_def unitary_sandwich_register)
+    have \<open>I o (F;G) = id\<close> and FGI: \<open>(F;G) o I = id\<close>
+       apply (auto intro!:ext simp: I_def[abs_def] FG sandwich_apply)
+       apply (metis (no_types, opaque_lifting) \<open>unitary U\<close> isometryD cblinfun_assoc_left(1) cblinfun_compose_id_right cblinfun_compose_id_left unitary_isometry)
+      by (metis (no_types, lifting) \<open>unitary U\<close> cblinfun_assoc_left(1) cblinfun_compose_id_left cblinfun_compose_id_right unitaryD2)
+    then show \<open>iso_register (F;G)\<close>
+      by (auto intro!: iso_registerI)
+  qed
+  ultimately show ?thesis
+    apply (rule_tac exI[of _ G]) by (auto)
+qed
+
 end
